wip

compiler/backend/proofs/exh_reorderProofScript.sml
@@ -16,9 +16,7 @@ val MEM_size_mono_v1_size = Q.store_thm("MEM_size_mono_v1_size",
 `! a v env. MEM (a,v) env ==> v_size v  < 1 + v1_size env`,
    Induct_on `env`
    \\ rw [v_size_def]
-   >- (
-     rw [v_size_def] 
-   )
+   >- rw [v_size_def] 
    \\ res_tac 
    \\ rw []
 )
@@ -42,6 +40,15 @@ val compile_v_def = tDefine "compile_v" `
 val _ = export_rewrites ["compile_v_def"];
 
 val _ = overload_on ("compile_env", ``MAP \(tn, v). (tn, compile_v v)``);
+
+val ALOOKUP_compile_env = Q.store_thm ("ALOOKUP_compile_env",
+    `! env q x. 
+        (ALOOKUP (compile_env env) q) = OPTION_MAP compile_v (ALOOKUP env q)`,
+    Induct \\ rw []
+    \\ pairarg_tac
+    \\ fs []
+    \\ rw []
+)
 
 val compile_store_v_def = Define `
     (compile_store_v (Refv v) = Refv (compile_v v)) /\
@@ -82,7 +89,9 @@ fun (f $ x) = f x
 
 (*
 val (asl, w) = top_goal ();
+val goal = top_goal ();
 *)
+
 fun hd_compile_sing_tac (goal as (asl,w)) = 
     let 
        val t = find_term (can (match_term ``HD (exh_reorder$compile [e])``)) w;
@@ -100,17 +109,144 @@ val compile_cons = Q.store_thm ("compile_cons",
    \\ METIS_TAC [compile_singleton, HD]
 )
 
+fun app_compile_sing_tac (goal as (asl,w)) =
+    let 
+        val t = find_term (can (match_term 
+            ``(evaluate env s (exh_reorder$compile [e1] ++ exh_reorder$compile (e2::es)))``)) w;
+        val app_term = rand $ t;
+        val e1_term = rand $ rator $ rand $ rand $ rator app_term;
+        val e2_term = rand $ rator $ rand $ rand app_term;
+        in 
+                (
+                 rw [Once compile_cons, SimpR ``$++``]
+                 THEN rw [Once compile_cons, SimpR ``CONS``]
+                 THEN (strip_assume_tac $ SPEC e1_term compile_singleton)
+                 THEN (strip_assume_tac $ SPEC e2_term compile_singleton)
+                )
+                goal
+
+    end
+
 val compile_nil = save_thm ("compile_nil[simp]", EVAL ``exh_reorder$compile []``);
+
+val compile_app_tran = Q.store_thm ("compile_app_tran", 
+    `! x h. compile (x ++ h) = (compile x) ++ (compile h)`,
+    Induct_on `x`
+    \\ fs []
+    \\ rw [Once compile_cons] 
+    \\ hd_compile_sing_tac
+    \\ rw [Once compile_cons]
+)
+
+val rev_compile_compile_rev = Q.store_thm ("rev_compile_compile_rev", 
+    `! x. REVERSE (compile x) = compile (REVERSE x)`,
+    Induct
+    \\ fs []
+    \\ rw [Once compile_cons]
+    \\ hd_compile_sing_tac
+    \\ rw [EQ_SYM_EQ, REVERSE_DEF]
+    \\ rw [compile_app_tran]
+   )
+
+val map_reverse_reverse_map = Q.store_thm ("map_reverse_reverse_map", 
+    `! f l. REVERSE (MAP f l) = MAP f (REVERSE l)`,
+    Induct_on `l`
+    \\ fs [])
+
+
+val ALOOKUP_none_not_some = Q.store_thm ("ALOOKUP_none_not_some",
+    `! env n. (ALOOKUP env n = NONE) ==> (ALOOKUP env n = SOME x) ==> F`,
+    Induct_on `env`
+    \\ fs []
+)
+
+val MAP_FST_MAP_triple = Q.store_thm ("MAP_FST_MAP_triple",
+    `! a b c y l. (MAP FST (MAP (\(a,b,c). a, b, (y c)) l)) = (MAP FST l)`,
+    Induct_on `l`
+    \\ fs []
+    \\ rw []
+    \\ pairarg_tac
+    \\ fs []
+)
+
+val _ = temp_overload_on ("None",``NONE``)
+val _ = temp_overload_on ("Some",``SOME``)
+val _ = temp_overload_on ("Length",``LENGTH``)
+
+val find_match_aux_def = Define`
+    find_match_aux refs v [] i = NONE /\
+    find_match_aux refs v (p::ps) i = 
+        if ALL_DISTINCT (pat_bindings p []) then
+            case pmatch refs p v [] of
+            | Match env' => SOME i
+            | _ => find_match_aux refs v ps (SUC i)
+        else NONE
+    `
+
+val find_match_def = Define`
+    find_match refs v ps = 
+        find_match_aux refs v ps 0
+`
+
+(*connection between evaluate_match and find_match*)
+val evaluate_match_find_match_none = Q.store_thm ("evaluate_match_find_match",
+    `!i. find_match_aux s.refs v (MAP FST pes) i = NONE ==>
+            evaluate_match env s v pes = (s, Rerr(Rabort Rtype_error))
+            `,
+    Induct_on `pes`
+    \\ fs [find_match_aux_def, evaluate_def]
+    \\ Cases
+    \\ fs [evaluate_def]
+    \\ gen_tac \\ strip_tac
+    \\ simp [Once pmatch_nil]
+    \\ every_case_tac
+    \\ fs []
+    \\ res_tac 
+)
+
+(*connection between evaluate_match and find_match*)
+val evaluate_match_find_match_some = Q.store_thm ("evaluate_match_find_match",
+    `!n i. find_match_aux s.refs v (MAP FST pes) n = Some (n + i) ==>
+            (i < Length pes /\
+            ? env'. pmatch s.refs (FST (EL i pes)) v env = 
+                Match env' /\
+                    evaluate_match env s v pes = evaluate env' s [(SND (EL i pes))])
+            `,
+    Induct_on `pes`
+    \\ fs [find_match_aux_def, evaluate_def]
+    \\ Cases
+    \\ fs [evaluate_def]
+    \\ ntac 2 gen_tac 
+    \\ fs [ADD1]
+    \\ TOP_CASE_TAC
+    here...
+    does i = 0 ?? is that insane ? 
+     
+    \\ strip_tac
+    \\ simp [Once pmatch_nil]
+    \\ every_case_tac
+    \\ fs []
+    \\ res_tac 
+)
+
+
+(*prove the connection to const_fst*)
+
+        
+    
+`
 
 val compile_correct = Q.store_thm( "compile_correct",
     `(!env ^s es s1 r1. 
-        (evaluate env s es = (s1, r1)) ==>
+        (evaluate env s es = (s1, r1)) /\
+        r1 <> Rerr (Rabort Rtype_error) ==>
         (evaluate (compile_env env) (compile_state s) (compile es) =
             (compile_state s1, map_result (MAP compile_v) compile_v r1)
             ))
        /\ 
         (!env ^s err_v pes s1 r1. 
-            evaluate_match env s err_v pes = (s1, r1) ==>
+            evaluate_match env s err_v pes = (s1, r1) /\
+            r1 <> Rerr (Rabort Rtype_error) =>
             evaluate_match (compile_env env) (compile_state s) (compile_v err_v) (const_cons_fst pes) = 
               (compile_state s1, map_result (MAP compile_v) compile_v r1))`,
     
@@ -118,11 +254,104 @@ val compile_correct = Q.store_thm( "compile_correct",
     \\ rw [compile_def] 
     \\ fs [evaluate_def]
     \\ rw []
-    \\ fs []
+    \\ fs [MAP_FST_MAP_triple]
+    (*17 subgoals*)
     >- (
-        (*step case (?) *)
+        (*step case ? *)
         every_case_tac
-        >- 
+        \\ fs []
+        \\ rfs []
+        \\ app_compile_sing_tac
+        \\ fs []
+        \\ rfs []
+        \\ rfs [Once compile_cons]
+        \\ imp_res_tac evaluate_sing
+        \\ rw []
+        \\ fs []
+        \\ rfs [Once evaluate_def]
+       )
+    (*16 subgoals left*)
+   >- (
+       hd_compile_sing_tac
+       \\ every_case_tac \\ fs [] \\ rw [] \\ rfs []
+       \\ imp_res_tac evaluate_sing \\ fs []
+   )
+   >- (
+      hd_compile_sing_tac
+      \\ every_case_tac \\ fs [] \\ rw [] \\ rfs []
+   )
+   >- (
+      every_case_tac \\ fs [] \\ rw [] \\ rfs []
+      \\ rfs [rev_compile_compile_rev]
+      \\ rw [map_reverse_reverse_map]
+      \\ fs [ETA_AX]
+   )
+   (*13 subgoals left...*)
+   >- (
+      every_case_tac \\ fs [ALOOKUP_compile_env]  
+   )
+   (* 12 subgoals *)
+   >- (
+      rfs [EL_MAP]
+      \\ fs [IS_SOME_EXISTS]
+   )
+   >- (
+      rfs [EL_MAP]
+   )
+   (*10*)
+   >- (
+      fs [EL_MAP]
+      \\ fs [IS_SOME_EXISTS]
+      \\ fs []
+   )
+
+   r 1
+  (*9*)
+   >- (
+      (*the app case*)
+      every_case_tac  \\ fs [rev_compile_compile_rev] \\ rfs []  \\ rw [compile_state_def]
+      (*32 subgoals...*)
+      >- (
+         \\ fs [] \\ rfs []
+         \\ rw []
+         \\ Induct_on `a'`
+         \\ fs []
+         \\ rw []
+         \\ rw [do_opapp_def]
+         \\ fs []
+         \\ rw []
+         \\ every_case_tac
+         >- (
+            fs [REVERSE_APPEND] \\ rfs [] \\ rw []
+            \\ fs [do_opapp_def]
+         )
+         >- (
+            fs []
+            \\ fs [do_opapp_def] 
+            \\ rw []
+            \\ res_tac 
+         )
+        
+   )
+   )
+   
+   >- (
+    (*the match case*)
+
+   )
+   >- (
+      fs [compile_state_def,MAP_GENLIST]
+   )
+   >- (
+     fs [const_cons_fst_def,const_cons_sep_def]
+     \\ fs [evaluate_def]
+   )
+   >-(
+    (*The actual pattern matching case*)
+
+   )
+        (*
+         >- 
         (
             fs []
             \\ rw []
@@ -140,6 +369,48 @@ val compile_correct = Q.store_thm( "compile_correct",
             \\ fs []
             \\ imp_res_tac evaluate_sing
             \\ rw []
+            \\ fs []
+        )
+        *)
+
+        >- 
+        (
+            app_compile_sing_tac
+            \\ fs []
+            \\ rfs []
+            \\ rfs [Once compile_cons]
+            \\ imp_res_tac evaluate_sing
+            \\ rw []
+            \\ fs []
+            \\ rfs [Once evaluate_def]
+        )
+        >- 
+        (
+            app_compile_sing_tac
+            \\ rw [Once evaluate_def]
+            \\ fs []
+        )
+        >- 
+        (
+            \\ fs []
+            \\ rw []
+            \\ res_tac
+            \\ app_compile_sing_tac
+            \\ rw [] 
+            \\ rw [Once evaluate_def]
+            \\ rfs []
+            \\ rw []
+            \\ rw [Once evaluate_def]
+            \\ fs []
+            \\ fs [Once compile_cons]
+        )
+        >-
+        (
+            fs []
+            \\ rw []
+            \\ app_compile_sing_tac
+            \\ rw []
+            \\ rw [Once evaluate_def]
             \\ fs []
         )
     )
